deps/poulet4/lib/P4cub/Semantics/Static/Auxiliary.v
@@ -1,21 +1,69 @@
+Require Import Coq.NArith.BinNat.
 From Poulet4 Require Export
      P4cub.Semantics.Static.Typing
      P4cub.Semantics.Static.IndPrincip
      P4cub.Semantics.Static.Util
      Utils.ForallMap.
 
-Local Hint Constructors t_ok : core.
+Ltac inv_numeric_width :=
+  match goal with
+  | H: numeric_width _ _ |- _ => inv H
+  end.
+
+Ltac inv_numeric :=
+  match goal with
+  | H: numeric _ |- _ => inv H; try inv_numeric_width
+  end.
+
+Ltac invert_type_expr :=
+  match goal with
+  | H: _ ⊢ₑ _ ∈ _ |- _ => inv H
+  end.
+
+Ltac invert_type_lists_ok :=
+  match goal with
+  | H: type_lists_ok _ _ _ |- _ => inv H
+  end.
+
+Section Lemmas.
+  Local Hint Resolve type_lists : core.
+  Local Hint Constructors type_lists_ok : core.
+  Local Hint Constructors t_ok_lists : core.
+
+  Lemma type_array : forall Γ τ es,
+      t_ok (type_vars Γ) τ ->
+      Forall (fun e => Γ ⊢ₑ e ∈ τ) es ->
+      Γ ⊢ₑ Expr.Lists (Expr.lists_array τ) es
+        ∈ Expr.TArray (N.of_nat (length es)) τ.
+  Proof.
+    intros G t es tok Hes; econstructor; eauto.
+    rewrite Nnat.Nat2N.id.
+    auto using Forall2_repeat_r.
+  Qed.
+
+  Lemma type_struct : forall Γ es τs,
+      Forall2 (type_expr Γ) es τs ->
+      Γ ⊢ₑ Expr.Lists Expr.lists_struct es ∈ Expr.TStruct false τs.
+  Proof. eauto. Qed.
+
+  Lemma type_header : forall Γ b es τs,
+      Forall2 (type_expr Γ) es τs ->
+      Γ ⊢ₑ Expr.Lists (Expr.lists_header b) es ∈ Expr.TStruct true τs.
+  Proof. eauto. Qed.
+
+  Local Hint Constructors t_ok : core.
   
-Lemma type_expr_t_ok : forall Γ e τ,
-    Γ ⊢ₑ e ∈ τ ->
-    Forall (t_ok (type_vars Γ)) (types Γ) ->
-    t_ok (type_vars Γ) τ.
-Proof.
-  intros G e t het hok;
-    induction het using custom_type_expr_ind; auto.
-  apply Forall2_only_r_Forall in H2.
-  rewrite Forall_forall in H2.
-  pose proof (fun t hin => H2 t hin hok) as h; clear H2.
-  rewrite <- Forall_forall in h.
-  inv H; inv H0; auto.
-Qed.
+  Lemma type_expr_t_ok : forall Γ e τ,
+      Γ ⊢ₑ e ∈ τ ->
+      Forall (t_ok (type_vars Γ)) (types Γ) ->
+      t_ok (type_vars Γ) τ.
+  Proof.
+    intros G e t het hok;
+      induction het using custom_type_expr_ind; auto.
+    apply Forall2_only_r_Forall in H2.
+    rewrite Forall_forall in H2.
+    pose proof (fun t hin => H2 t hin hok) as h; clear H2.
+    rewrite <- Forall_forall in h.
+    inv H; inv H0; auto.
+  Qed.
+End Lemmas.
